extraction/theories/Certifying.v
@@ -1,0 +1,109 @@
+From Coq Require Import List PeanoNat Bool Ascii String.
+From MetaCoq.Template Require Import Kernames All Ast.
+From ConCert.Extraction Require Import ResultMonad.
+From ConCert.Utils Require StringExtra.
+
+
+Open Scope string.
+
+Import ListNotations.
+Import MonadNotation.
+
+Definition get_def_name (name : kername) : string :=
+  StringExtra.replace_char "." "_" (string_of_kername name).
+
+Definition change_modpath (mpath : modpath) (suffix : string) (expansion_ignore : kername -> bool)
+  : term -> term :=
+  fix go (t : term) : term :=
+    match t with
+    | tRel n => t
+    | tVar id => t
+    | tSort s => t
+    | tEvar ev args => tEvar ev (map (go) args)
+    | tCast t kind v => tCast (go t) kind (go v)
+    | tProd na ty body => tProd na (go ty) (go body)
+    | tLambda na ty body => tLambda na (go ty) (go body)
+    | tLetIn na def def_ty body =>
+      tLetIn na (go def) (go def_ty) (go body)
+    | tApp f args => tApp (go f) (map (go) args)
+    | tConst kn u => if expansion_ignore kn then t
+                    else tConst (mpath, get_def_name kn ++ suffix) u
+    | tInd ind u => t
+    | tConstruct ind idx u => t
+    | tCase ind_and_nbparams type_info discr branches =>
+      tCase ind_and_nbparams (go type_info)
+            (go discr) (map (on_snd (go)) branches)
+    | tProj proj t => tProj proj (go t)
+    | tFix mfix idx => tFix (map (map_def (go) (go)) mfix) idx
+    | tCoFix mfix idx => tCoFix (map (map_def (go) (go)) mfix) idx
+    | tInt _ => t
+    | tFloat _ => t
+  end.
+
+Fixpoint map_constants_global_env (k : kername -> kername) (f : constant_body -> constant_body) (Σ : global_env) : global_env :=
+  match Σ with
+  | [] => []
+  | (kn, ConstantDecl cb) :: Σ' => (k kn, ConstantDecl (f cb)) :: map_constants_global_env k f Σ'
+  | gd :: Σ' => gd :: map_constants_global_env k f Σ'
+  end.
+
+Definition add_suffix_global_env (mpath : modpath) (suffix : string) (expansion_ignore : kername -> bool) (Σ : global_env) :=
+  map_constants_global_env
+    (fun kn => (mpath,get_def_name kn ++ suffix))
+    (fun cb => {| cst_type := cb.(cst_type);
+               cst_body := b <- cb.(cst_body);;
+                           Some (change_modpath mpath suffix expansion_ignore b);
+               cst_universes := cb.(cst_universes) |}) Σ.
+
+
+Definition generate_proof (Σ1 Σ2 : global_env) (kn1 kn2 : kername) : TemplateMonad (term × term × term × term) :=
+  match lookup_env Σ1 kn1, lookup_env Σ2 kn2  with
+  | Some (ConstantDecl cb1), Some (ConstantDecl cb2) =>
+    match cb1.(cst_body), cb2.(cst_body) with
+    | Some _, Some exp_body =>
+      let ty := cb1.(cst_type) in
+      let proof_ty :=
+          tApp (tInd
+                  {| inductive_mind := (MPfile ["Logic"; "Init"; "Coq"], "eq");
+                     inductive_ind := 0 |} [])
+               [ty; tConst kn1 []; tConst kn2 []] in
+      let proof_body := tApp (tConstruct
+                          {| inductive_mind := (MPfile ["Logic"; "Init"; "Coq"], "eq");
+                             inductive_ind := 0 |} 0 [])
+                       [ty;tConst kn1 []] in
+      ret (cb1.(cst_type), (exp_body, (proof_ty, proof_body)))
+    | _,_ => tmFail "No body"
+    end
+  | None, _ => tmFail ("Not found: " ++ kn1.2)
+  | _, None => tmFail ("Not found: " ++ kn2.2)
+  | _,_ => tmFail "Not a constant"
+  end.
+
+Definition gen_proof_prog (Σ1 Σ2 : global_env) (kn1 kn2 : kername) : TemplateMonad unit :=
+  '(exp_ty, (exp_t, (p_ty, p_t))) <- generate_proof Σ1 Σ2 kn1 kn2 ;;
+  tmBind (tmUnquoteTyped Type exp_ty)
+         (fun A => ucst <- tmUnquoteTyped A exp_t ;;
+                 tmDefinition kn2.2 ucst;;
+            tmBind (tmUnquoteTyped Type p_ty)
+                   (fun B =>
+                      uproof <- tmUnquoteTyped B p_t ;;
+                      tmDefinition (kn2.2 ++ "_correct") uproof ;;
+                      tmPrint B)).
+
+Definition is_none {A} (o : option A) :=
+  match o with
+  | Some _ => false
+  | None => true
+  end.
+
+Definition gen_defs_and_proofs (Σ : global_env) (mpath : modpath) (suffix: string) (ignore : kername -> bool)  : TemplateMonad unit :=
+  let Σdecls := filter (fun '(kn,gd) => match gd with
+                                    | ConstantDecl cb => negb (is_none cb.(cst_body))
+                                    | _ => false
+                                     end) Σ in
+  Σdecls' <- tmEval lazy (add_suffix_global_env mpath suffix ignore Σdecls) ;;
+  monad_iter (fun kn1 =>
+                if ignore kn1 then ret tt
+                else
+                  gen_proof_prog Σ Σdecls' kn1 (mpath, get_def_name kn1 ++ suffix))
+             (List.rev (map fst Σdecls)).
